

Logarithms.

$$3^4 = 81 \Leftrightarrow \log_3 81 = 4$$

$$N = a^x.$$

$$N > 0 : a > 0 : a \neq 1.$$

$$a^x = N \Leftrightarrow x = \log_a (N)$$

$$a^x = (N) \Leftrightarrow x = \log_a N$$

$$10^2 = 100$$

$$\Leftrightarrow \log_{10} 100 = 2$$

$$(0.1)^3 = 0.001$$

$$\Leftrightarrow \log_{0.1} 0.001 = 3$$

$$2^4 = 16 \Leftrightarrow \log_2 16 = 4$$

$$3^3 = 27 \Leftrightarrow \log_3 27 = 3$$

$$a^x = N > 0 \Leftrightarrow \log_{\textcircled{a}} \textcircled{N} = x$$

$a > 0; a \neq 1$

$$N > 0; a > 0; a \neq 1$$

$$10^1 = 10 \Leftrightarrow \log_{10} 10 = 1$$

$$a^1 = a \Leftrightarrow \log_a a = 1$$

$$\log_a a = 1$$

$a > 0; a \neq 1$

$$a^0 = 1 \Leftrightarrow \log_a 1 = 0$$

$$\log_a 1 = 0 \quad (a > 0 : a \neq 1)$$

$$\log_a a = 1.$$

$$\log_{\frac{1}{a}} a =$$

- 1) $\log_N N = 1$
- 2) $\log_N 1 = 0$
- 3) $\log_{\frac{1}{N}} N = \log_N \frac{1}{N} = -1$

$$a^{-1} = \frac{1}{a}.$$

$$\Leftrightarrow \log_a \left(\frac{1}{a}\right) = -1.$$

$$\Leftrightarrow \log_{\frac{1}{a}} a = -1$$

$$a^x = N \Rightarrow \log_a N = x$$

then N is Anti log of x to the base a .

$$2^3 = 8 \Leftrightarrow \log_2 8 = 3$$

$8 =$ Anti log of 3 with base 2 .

Prob.:

Anti log of $\left(\frac{5}{6}\right)$ with base $\frac{6}{5}$.

$$= \left(\frac{6}{5}\right)^{\frac{5}{6}} = 2^5 = \boxed{32}$$

Find Anti log of $\frac{2}{3}$ with base 27

$$(27)^{\frac{2}{3}} = (3^3)^{\frac{2}{3}} = 3^2 = \boxed{9}$$

Properties: 1) $\log_a m + \log_a n = \log_a (mn)$

$$m, n > 0 : a > 0, a \neq 1$$

$$2) \log_a \left(\frac{m}{n} \right) = \log_a m - \log_a n$$

$$3) \log_a a^x = x \cdot \log_a a$$

$$\log_b a^x = x \log_b a$$

$$\text{L.H.S} = \log_b a^x = K.$$

$$a^x = b^K.$$

$$a = (b^K)^{1/x}.$$

$$a = b^{\frac{K}{x}}.$$

$$\text{R.H.S} = x \cdot \log_b b^{\frac{K}{x}}.$$

$$= x \cdot \frac{K}{x} \log_b b.$$

$$= \boxed{K}.$$

$$\text{L.H.S} = \text{R.H.S}.$$

$$\log_{a^m} N = \frac{1}{m} \log_a N$$

Ex: $\log_{16} 2^4 = \log_{16} 16 = 1$

$$\log_{16} 2 = \log_{2^4} 2 = \frac{1}{4} \log_2 2 = \boxed{\frac{1}{4}}$$

$$\log_3 3^5 = 5 \cdot \log_3 3 = \boxed{5}$$

$$a^{\log_a N} = N$$

$$\Leftrightarrow \log_a N = \log_a N$$

$$Q. \log_c b = x \Rightarrow b = c^x$$

$$\text{Take } \log_c b = x$$

$$\Rightarrow b = c^x$$

$$L.H.S = c^x$$

$$(a^m)^n = a^{mn}$$

$$R.H.S = b^{\log_c a}$$

$$= (c^x)^{\log_c a}$$

$$= c^{x \log_c a}$$

$$= c^{\log_c (a^x)}$$

$$= a^x$$

$$\therefore L.H.S = R.H.S$$

$$1) \log_4 m = 1.5 \Rightarrow m = \underline{\hspace{2cm}}$$

$$m = 4^{1.5} \\ = (2^2)^{3/2} = 2^3 = \boxed{8}$$

$$1728 = (12)^3 \\ = (2^2 \cdot 3)^3$$

$$2) \log_{2\sqrt{3}} 1728 = x \Rightarrow x = \underline{\hspace{2cm}}$$

$$1728 = (2\sqrt{3})^x \\ (2^2 \cdot 3)^3 = (2\sqrt{3})^x \Rightarrow \boxed{x=6}$$

$$\log_a \left[1 + \log_b \left\{ 1 + \log_c \left(1 + \log_p N \right) \right\} \right] = 0$$

Then $N = \underline{\hspace{2cm}}$

Sol.:

$$\cancel{1 + \log_b \left\{ 1 + \log_c \left(1 + \log_p N \right) \right\}} = \cancel{x}$$

$$\cancel{1 + \log_c \left(1 + \log_p N \right)} = \cancel{1^0} = \cancel{x}$$

$$\cancel{\left(1 + \log_p N \right)} = \cancel{x}$$

$$N = p^0 = 1.$$

$$\log_a \left[1 + \log_b \left\{ 1 + \log_c \left(1 + \log_p N \right) \right\} \right] = 0$$

$$\cancel{1 + \log_b \left\{ 1 + \log_c \left(1 + \log_p N \right) \right\} = a^0 = 1}$$

$$\log_p N = 0$$

$$N = p^0$$

$$= 1$$

$$\log_b \left\{ 1 + \log_c \left(1 + \log_p N \right) \right\} = 0$$

$$\cancel{1 + \log_c \left(1 + \log_p N \right) = 1}$$

$$\log_c \left(1 + \log_p N \right) = 0$$

$$\cancel{1 + \log_p N = 1}$$

$$4^{\log_2 2x} = 36 \Rightarrow x = \text{---}$$

$$\left(\frac{2}{2}\right)^{\log_2 2x} = 36$$

$$2^{2 \log_2 2x} = 36$$

$$2^{\log_2 4x^2} = 36$$

$$4x^2 = 36$$

$$\Rightarrow \boxed{x=3}$$

$$\left(\frac{1}{2}\right)^{\log_2 5} = \underline{\hspace{2cm}}.$$

$$\left(2^{-1}\right)^{\log_2 5} = 2^{-\log_2 5}$$

$$= 2^{\log_2 5^{-1}}$$

$$= 5^{-1} = \boxed{\frac{1}{5}}$$

$$1) \quad \text{If } a^2 + b^2 = 23ab \text{ then } \log \left(\frac{a+b}{5} \right) = \underline{\hspace{2cm}}$$

$$a^2 + b^2 + 2ab = 25ab.$$

$$(a+b)^2 = 5^2 ab.$$

$$\frac{a^m}{b^m} = \left(\frac{a}{b} \right)^m$$

$$\left(\frac{a+b}{5} \right)^2 = ab. \Rightarrow \log \left(\frac{a+b}{5} \right)^2 = \log ab$$

$$2 \log \left(\frac{a+b}{5} \right) = \log a + \log b$$

$$\log \left(\frac{a+b}{5} \right) = \boxed{\frac{1}{2} [\log a + \log b]}$$

Simplify

$$\frac{1}{2} \log 9 + 2 \log 6 + \frac{1}{4} \log 81 - \log 12.$$

= _____

Sol:

$$\frac{1}{2} \log 3^2 + 2[\log 3 + \log 2] + \frac{1}{4} \log 3^4$$

$$= [\log 2^2 \cdot 3]$$

$$= \cancel{2} \times \frac{1}{2} \log 3 + 2 \log 3 + 2 \log 2 + \cancel{4} \times \frac{1}{4} \log 3$$

$$= 4 \log 3 + \cancel{2 \log 2} - \cancel{2 \log 2} - \log 2^2 - \log 3$$

$$= 3 \log 3$$

If $\log_e x - \log_e y = a$: $\log_e y - \log_e z = b$:

$\log_e z - \log_e x = c$

then $\left(\frac{x}{y}\right)^{b-c} \cdot \left(\frac{y}{z}\right)^{c-a} \cdot \left(\frac{z}{x}\right)^{a-b} = \underline{\hspace{2cm}}$

Sol: $\log_e \left(\frac{x}{y}\right) = a \Rightarrow \frac{x}{y} = e^a$

$\implies \left(\frac{x}{y}\right)^{b-c} = (e^a)^{b-c} = e^{ab-ac}$

$\implies \left(\frac{y}{z}\right)^{c-a} = e^{bc-ba}$: $\left(\frac{z}{x}\right)^{a-b} = e^{ac-bc}$

~~$e^{ab-ac+bc-ba+ac-bc}$~~
 $e^0 = 1$

Base changing property

$$\log_a N = \frac{\log_b N}{\log_b a} = \frac{\log_c N}{\log_c a} = \frac{\log_d N}{\log_d a}$$

$$b, c, d, \dots > 0$$

$$b, c, d \neq 1.$$

$$\log_e x = \log_e x = \ln x \quad (\text{Natural logarithm})$$

$$\log_{10} x \quad (\text{Common logarithms})$$

$$\log_b a \cdot \log_c b$$

$$= \log_c a$$

$$\log_e x \times \log_{10} e = \log_{10} x$$

$$\log_e x \times 0.4342$$

$$= \log_{10} x$$

$$\log_a N = \frac{\log_b N}{\log_b a}$$

$$\log_{10} x \cdot \log_e 10$$

$$\log_{10} x$$

$$\log_{10} e$$

$$2.303 \checkmark$$

$$= \frac{\log_e N}{\log_e a} = \frac{\log N \cdot}{\log a \cdot}$$

$$= \frac{\log x}{\cancel{\log 10}} \times \frac{\cancel{\log 10}}{\log e}$$

$$= \frac{\log x}{\log e} = \log_e x$$

$$= \log_e x$$

$$\log_e x \times \log_{10} e = \log_{10} x$$

$$\log_e x \times 0.4342 = \log_{10} x$$

